theories/L3_flattenedApp/term.v
@@ -51,7 +51,7 @@ apply TrmTrmsDefs_ind.
   [lft | rght .. ].
 - induction t1; cross.
   destruct p as [n l], p0 as [n0 l0].
-  destruct (eq_nat_dec n n0); destruct (nat_list_dec l l0);
+  destruct (eq_dec n n0); destruct (nat_list_dec l l0);
   destruct (H t1); destruct (H0 t2);
   [lft | rght .. ].
 - induction t; cross.
@@ -572,7 +572,7 @@ Qed.
 Function instantiate (n:nat) (tbod:Term) {struct tbod} : Term :=
   match tbod with
     | TRel m => match nat_compare n m with
-                  | Eq => tin
+                  | Datatypes.Eq => tin
                   | Gt => TRel m
                   | Lt => TRel (pred m)
                 end
